Progress on Blake2s

code/hash/Hacl.Impl.Blake2s.fst
@@ -24,11 +24,19 @@ inline_for_extraction let v = size_v
 inline_for_extraction let index (x:size_nat) = size x
 let op_String_Access #a #len m b = as_lseq #a #len b m
 
+///
+/// Helper lemmata
+///
 
 val lemma_cast_to_u64: x:uint32 -> Lemma
   (requires (True))
   (ensures  (to_u64 #U32 x == u64 (uint_v #U32 x)))
 let lemma_cast_to_u64 x = admit()
+
+val lemma_modifies0_is_modifies2: #a0:Type -> #a1:Type -> #len0:size_nat -> #len1:size_nat -> b0:lbuffer a0 len0 -> b1:lbuffer a1 len1 -> h0:mem -> h1:mem -> Lemma
+  (requires (True))
+  (ensures  (h0 == h1 ==> modifies2 b0 b1 h0 h1))
+let lemma_modifies0_is_modifies2 #a0 #a1 #len0 #len1 b0 b1 h0 h1 = admit()
 
 val lemma_repeati: #a:Type -> n:size_nat -> f:(i:size_nat{i < n}  -> a -> Tot a) -> init:a -> i:size_nat{i < n} -> Lemma
   (requires True)
@@ -341,7 +349,7 @@ let blake2s_internal1 s kk nn =
 
 #reset-options "--max_fuel 0 --z3rlimit 25"
 
-val blake2s_internal2_: s:lbuffer uint32 8 ->
+val blake2s_internal2_inner: s:lbuffer uint32 8 ->
    dd:size_t{0 < size_v dd /\ size_v dd * Spec.bytes_in_block <= max_size_t}  ->
    d:lbuffer uint8 (size_v dd * Spec.bytes_in_block) ->
    to_compress:lbuffer uint32 16 ->
@@ -356,63 +364,52 @@ val blake2s_internal2_: s:lbuffer uint32 8 ->
                     /\ disjoint d to_compress /\ disjoint to_compress d /\ disjoint to_compress const_sigma /\ disjoint const_sigma to_compress
                     /\ disjoint to_compress const_iv /\ disjoint const_iv to_compress))
      (ensures  (fun h0 _ h1 -> preserves_live h0 h1 /\ modifies2 s to_compress h0 h1
-                          /\ h1.[s] == Spec.blake2s_internal2_ (v dd) h0.[d] (v i) h0.[s]))
+                          /\ h1.[s] == Spec.blake2s_internal2_inner (v dd) h0.[d] (v i) h0.[s]))
 
 [@ Substitute]
-let blake2s_internal2_ s dd d to_compress i const_iv const_sigma =
+let blake2s_internal2_inner s dd d to_compress i const_iv const_sigma =
   let sub_d = sub d (i *. (size Spec.bytes_in_block)) (size Spec.bytes_in_block) in
   uint32s_from_bytes_le #16 (size 16) to_compress sub_d;
   let offset32 = size_to_uint32 ((i +. (size 1)) *. (size Spec.block_bytes)) in
   let offset = to_u64 #U32 offset32 in
-  lemma_cast_to_u64 offset32;
+  (**) lemma_cast_to_u64 offset32;
   blake2_compress s to_compress offset false const_iv const_sigma
 
 
-// val blake2s_internal2_alloc: s:lbuffer uint32 8 ->
-//    dd:size_t{0 < size_v dd /\ size_v dd * Spec.bytes_in_block <= max_size_t}  ->
-//    d:lbuffer uint8 (size_v dd * Spec.bytes_in_block) ->
-//    i:size_t{v i < v dd - 1} ->
-//    const_iv:init_vector -> const_sigma:sigma_t ->
-//    Stack unit
-//      (requires (fun h -> live h s /\ live h d /\ live h const_iv /\ live h const_sigma
-//                     /\ h.[const_sigma] == Spec.sigma
-//                     /\ h.[const_iv] == Spec.const_init
-//                     /\ disjoint s d /\ disjoint s const_iv /\ disjoint s const_sigma
-//                     /\ disjoint d s /\ disjoint const_iv s /\ disjoint const_sigma s))
-//      (ensures  (fun h0 _ h1 -> preserves_live h0 h1 /\ modifies1 s h0 h1
-//                           /\ h1.[s] == Spec.blake2s_internal2_ (v dd) h0.[d] (v i) h0.[s]))
+val blake2s_internal2_loop: s:lbuffer uint32 8 ->
+   dd:size_t{0 < size_v dd /\ size_v dd * Spec.bytes_in_block <= max_size_t}  ->
+   d:lbuffer uint8 (size_v dd * Spec.bytes_in_block) ->
+   to_compress:lbuffer uint32 16 ->
+   const_iv:init_vector -> const_sigma:sigma_t ->
+   Stack unit
+     (requires (fun h -> live h s /\ live h d /\ live h to_compress /\ live h const_iv /\ live h const_sigma
+                    /\ h.[const_sigma] == Spec.sigma
+                    /\ h.[const_iv] == Spec.const_init
+                    // Disjointness for s
+                    /\ disjoint s d /\ disjoint d s
+                    /\ disjoint s const_iv /\ disjoint const_iv s
+                    /\ disjoint s const_sigma /\ disjoint const_sigma s
+                    // Disjointness for to_compress
+                    /\ disjoint to_compress d /\ disjoint d to_compress
+                    /\ disjoint to_compress const_iv /\ disjoint const_iv to_compress
+                    /\ disjoint to_compress const_sigma /\ disjoint const_sigma to_compress
+                    // Disjointness for s and to_compress
+                    /\ disjoint s to_compress /\ disjoint to_compress s))
+     (ensures  (fun h0 _ h1 -> preserves_live h0 h1 /\ modifies2 s to_compress h0 h1
+                          /\ h1.[s] == Spec.blake2s_internal2_loop (v dd) h0.[d] h0.[s]))
 
-// [@ Substitute]
-// let blake2s_internal2_alloc s dd d i const_iv const_sigma =
-//   (**) let hi = ST.get () in
-//   // let f h0 h1 = (h1.[s] == Spec.blake2s_internal2_ (v dd) h0.[d] (v i) h0.[s]) in
-//   salloc' #hi #_ #_ #16 (size 16) (u32 0) [BufItem d; BufItem const_iv; BufItem const_sigma] [BufItem s]
-//   (fun h0 _ h1 -> (h1.[s] == Spec.blake2s_internal2_ (v dd) h0.[d] (v i) h0.[s]))
-//   (fun m ->
-//     let h0 = ST.get () in
-//     assert(h0.[const_sigma] == Spec.sigma /\ h0.[const_iv] == Spec.const_init);
-//     blake2s_internal2_ s dd d m i const_iv const_sigma)
-//     //let h1 = ST.get () in
-//     // TODO: This is very wrong ! :)
-//     // Lemmas on alloc() seem to trigger when impl is modifies1 but not when it is a modifies2.
-//     // assume(modifies1 s h0 h1))
-
-
-// val blake2s_internal2: s:lbuffer uint32 8 ->
-//    dd:size_t{0 < size_v dd /\ size_v dd * Spec.bytes_in_block <= max_size_t}  ->
-//    d:lbuffer uint8 (size_v dd * Spec.bytes_in_block) -> to_compress:lbuffer uint32 16 ->
-//    const_iv:init_vector -> const_sigma:sigma_t ->
-//    Stack unit
-//      (requires (fun h -> live h s /\ live h d /\ live h const_iv /\ live h const_sigma
-//                     /\ h.[const_sigma] == Spec.sigma
-//                     /\ h.[const_iv] == Spec.const_init
-//                     /\ disjoint s d /\ disjoint s const_iv /\ disjoint s const_sigma
-//                     /\ disjoint d s /\ disjoint const_iv s /\ disjoint const_sigma s))
-//      (ensures  (fun h0 _ h1 -> preserves_live h0 h1 /\ modifies1 s h0 h1
-//                           /\ h1.[s] == Spec.blake2s_internal2  (v dd) h0.[d] h0.[s]))
-
-
-
+[@ Substitute]
+let blake2s_internal2_loop s dd d to_compress const_iv const_sigma =
+  (**) let h0 = ST.get () in
+  let spec hi =
+    let s0 = h0.[s] in
+    let d0 = h0.[d] in
+    Spec.blake2s_internal2_inner (v dd) d0 in
+  let idx = dd -. (size 1) in
+  loop #h0 idx s spec
+  (fun i ->
+     blake2s_internal2_inner s dd d to_compress i const_iv const_sigma;
+     lemma_repeati (v idx) (spec h0) h0.[s] (v i))
 
 val blake2s_internal2: s:lbuffer uint32 8 ->
    dd:size_t{0 < size_v dd /\ size_v dd * Spec.bytes_in_block <= max_size_t}  ->
@@ -423,28 +420,28 @@ val blake2s_internal2: s:lbuffer uint32 8 ->
      (requires (fun h -> live h s /\ live h d /\ live h to_compress /\ live h const_iv /\ live h const_sigma
                     /\ h.[const_sigma] == Spec.sigma
                     /\ h.[const_iv] == Spec.const_init
-                    /\ disjoint s d /\ disjoint s to_compress /\ disjoint s const_iv /\ disjoint s const_sigma
-                    /\ disjoint d s /\ disjoint to_compress s /\ disjoint const_iv s /\ disjoint const_sigma s
-                    /\ disjoint d to_compress /\ disjoint to_compress d /\ disjoint to_compress const_sigma /\ disjoint const_sigma to_compress
-                    /\ disjoint to_compress const_iv /\ disjoint const_iv to_compress))
+                    // Disjointness for s
+                    /\ disjoint s d /\ disjoint d s
+                    /\ disjoint s const_iv /\ disjoint const_iv s
+                    /\ disjoint s const_sigma /\ disjoint const_sigma s
+                    // Disjointness for to_compress
+                    /\ disjoint to_compress d /\ disjoint d to_compress
+                    /\ disjoint to_compress const_iv /\ disjoint const_iv to_compress
+                    /\ disjoint to_compress const_sigma /\ disjoint const_sigma to_compress
+                    // Disjointness for s and to_compress
+                    /\ disjoint s to_compress /\ disjoint to_compress s))
      (ensures  (fun h0 _ h1 -> preserves_live h0 h1 /\ modifies2 s to_compress h0 h1
                           /\ h1.[s] == Spec.blake2s_internal2 (v dd) h0.[d] h0.[s]))
 
 [@ Substitute]
 let blake2s_internal2 s dd d to_compress const_iv const_sigma =
   (**) let h0 = ST.get () in
-  let spec hi =
-    let s0 = h0.[s] in
-    let d0 = h0.[d] in
-    Spec.blake2s_internal2_ (v dd) d0 in
-  if (dd >. size 1) then begin
-    let idx = dd -. (size 1) in
-    loop #h0 idx s spec
-    (fun i ->
-      blake2s_internal2_ s dd d to_compress i const_iv const_sigma;
-      lemma_repeati (v idx) (spec h0) h0.[s] (v i)
-    ) end
-   else ()
+  if (dd >. size 1) then
+    blake2s_internal2_loop s dd d to_compress const_iv const_sigma
+  else begin
+    (**) let h1 = ST.get () in
+    (**) lemma_modifies0_is_modifies2 s to_compress h0 h1
+  end
 
 
 val blake2s_internal3: s:lbuffer uint32 8 ->
@@ -458,7 +455,9 @@ val blake2s_internal3: s:lbuffer uint32 8 ->
                     /\ h.[const_sigma] == Spec.sigma
                     /\ h.[const_iv] == Spec.const_init
                     /\ disjoint s d /\ disjoint s to_compress /\ disjoint s tmp /\ disjoint s res /\ disjoint s const_iv /\ disjoint s const_sigma
-                    /\ disjoint d s /\ disjoint to_compress s /\ disjoint tmp s /\ disjoint res s /\ disjoint const_iv s /\ disjoint const_sigma s))
+                    /\ disjoint d s /\ disjoint to_compress s /\ disjoint tmp s /\ disjoint res s /\ disjoint const_iv s /\ disjoint const_sigma s
+                    /\ disjoint d to_compress /\ disjoint to_compress d /\ disjoint to_compress const_sigma /\ disjoint const_sigma to_compress
+                    /\ disjoint to_compress const_iv /\ disjoint const_iv to_compress))
      (ensures  (fun h0 _ h1 -> preserves_live h0 h1 /\ modifies1 res h0 h1
                           /\ h1.[res] == Spec.blake2s_internal3 h0.[s] (v dd) h0.[d] (v ll) (v kk) (v nn)))
 
@@ -466,7 +465,6 @@ val blake2s_internal3: s:lbuffer uint32 8 ->
 let blake2s_internal3 s dd d ll kk nn to_compress tmp res const_iv const_sigma =
   let offset:size_t = (dd -. (size 1)) *. (size 64) in
   let sub_d = sub d offset (size Spec.bytes_in_block) in
-  assert(false);
   uint32s_from_bytes_le (size 16) to_compress sub_d;
   (if kk =. size 0 then
     blake2_compress s to_compress (to_u64 #U32 (size_to_uint32 ll)) true const_iv const_sigma
@@ -498,6 +496,9 @@ val blake2s_internal:
                     /\ disjoint s tmp /\ disjoint s const_iv /\ disjoint s const_sigma
                     /\ disjoint d s /\ disjoint to_compress s /\ disjoint wv s
                     /\ disjoint tmp s /\ disjoint const_iv s /\ disjoint const_sigma s
+                    // Disjointness for to_compress
+                    /\ disjoint d to_compress /\ disjoint to_compress d /\ disjoint to_compress const_sigma /\ disjoint const_sigma to_compress
+                    /\ disjoint to_compress const_iv /\ disjoint const_iv to_compress
                     // Disjointness for res and s
                     /\ disjoint res s /\ disjoint s res))
      (ensures  (fun h0 _ h1 -> preserves_live h0 h1 /\ modifies2 res s h0 h1
